src/TacPackIL.v
@@ -1,0 +1,381 @@
+Require Import Expr SepExpr.
+Require Import Prover SymEval.
+Require Import Env TypedPackage.
+Import List.
+
+Require Import IL SepIL SymIL ILEnv.
+
+Set Implicit Arguments.
+Set Strict Implicit.
+Require Unfolder.
+Module UNF := Unfolder.Make SH ExprUnify.UNIFIER.
+Module PACKAGED := UNF.Packaged BedrockCoreEnv.
+Module PACK := PACKAGED.PACK.
+
+Module ILAlgoTypes <: AlgoTypes SEP BedrockCoreEnv.
+
+  Record AllAlgos (ts : list type) : Type :=
+  { Prover : option (ProverT (repr BedrockCoreEnv.core ts))
+  ; Hints : option (UNF.hintsPayload (repr BedrockCoreEnv.core ts) BedrockCoreEnv.pc BedrockCoreEnv.st)
+  ; MemEval : option (MEVAL.MemEvaluator (repr BedrockCoreEnv.core ts) BedrockCoreEnv.pc BedrockCoreEnv.st)
+  }.
+
+  Section oplus.
+    Variable T : Type.
+    Variable F : T -> T -> T.
+
+    Definition oplus (l r : option T) : option T :=
+      match l , r with 
+        | None , _ => r
+        | _ , None => l
+        | Some l , Some r => Some (F l r)
+      end.
+  End oplus.
+
+  Definition AllAlgos_composite types (l r : AllAlgos types) : AllAlgos types :=
+    match l , r with
+      | {| Prover  := pl ; Hints := hl ; MemEval := ml |} , {| Prover := pr ; Hints := hr ; MemEval := mr |} =>
+        {| Prover  := oplus (@composite_ProverT _) pl pr 
+         ; Hints   := oplus (fun l r => {| UNF.Forward := UNF.Forward l ++ UNF.Forward r
+         ; UNF.Backward := UNF.Backward l ++ UNF.Backward r |}) hl hr
+         ; MemEval := oplus (@MEVAL.Composite.MemEvaluator_composite _ BedrockCoreEnv.pc BedrockCoreEnv.st) ml mr
+        |}
+    end.
+
+  Record AllAlgos_correct
+    (types : list type)
+    (funcs : functions (repr BedrockCoreEnv.core types))
+    (preds : SEP.predicates (repr BedrockCoreEnv.core types) BedrockCoreEnv.pc BedrockCoreEnv.st)
+    (algos : AllAlgos types) : Type :=
+  { Acorrect_Prover :
+    match Prover algos with
+      | None => True
+      | Some P => ProverT_correct P funcs
+    end
+  ; Acorrect_Hints : 
+    match Hints algos with
+      | None => True
+      | Some H => UNF.hintsSoundness funcs preds H
+    end
+  ; Acorrect_MemEval :
+    match MemEval algos with
+      | None => True
+      | Some M => 
+        @MEVAL.MemEvaluator_correct _ BedrockCoreEnv.pc BedrockCoreEnv.st M funcs preds
+          (tvarD (repr BedrockCoreEnv.core types) BedrockCoreEnv.st) (tvType 0) (tvType 0) 
+          (@IL_mem_satisfies types) (@IL_ReadWord types) (@IL_WriteWord types)
+    end
+  }.
+
+  Theorem AllAlgos_correct_composite types (l r : AllAlgos types) funcs preds 
+    (CL : @AllAlgos_correct types funcs preds l)
+    (CR : @AllAlgos_correct types funcs preds r) :
+    @AllAlgos_correct types funcs preds (AllAlgos_composite l r).
+  Proof.
+    destruct l; destruct r; destruct CL; destruct CR; simpl in *; constructor; simpl.
+    destruct Prover0; destruct Prover1; simpl; auto. apply composite_ProverT_correct; auto.
+    destruct Hints0; destruct Hints1; simpl; auto; destruct Acorrect_Hints0; destruct Acorrect_Hints1; constructor; simpl;
+      eapply Folds.Forall_app; auto.
+    destruct MemEval0; destruct MemEval1; simpl; auto. apply MEVAL.Composite.MemEvaluator_correct_composite; auto.
+  Qed.
+
+  Record TypedPackage : Type :=
+  { Env   : PACK.TypeEnv
+  ; Algos : forall ts, AllAlgos (PACK.applyTypes Env ts)
+  ; Algos_correct : forall ts fs ps,
+    @AllAlgos_correct (PACK.applyTypes Env ts) (PACK.applyFuncs Env _ fs) (PACK.applyPreds Env _ ps) (Algos ts)
+  }.
+
+  Definition EnvOf : TypedPackage -> PACK.TypeEnv := Env.
+
+  Module EmptyPackage.
+    Definition empty_package : TypedPackage.
+    refine (
+      {| Env := {| PACK.Types := nil_Repr EmptySet_type
+                 ; PACK.Funcs := fun ts => nil_Repr (Default_signature _)
+                 ; PACK.Preds := fun ts => nil_Repr (SEP.Default_predicate _ _ _)
+                |} 
+       ; Algos := fun ts => {| Prover := None ; Hints := None ; MemEval := None |}
+       ; Algos_correct := _
+      |}).
+    abstract (constructor; simpl; trivial).
+    Defined.
+  
+(*
+    Ltac simplifier s1 s2 s3 H :=
+      match H with
+        | tt => 
+          cbv delta [ s1 s2 s3
+            empty_package UNF.default_hintsPayload
+          ]
+        | _ => 
+          cbv delta [ s1 s2 s3
+            empty_package UNF.default_hintsPayload
+          ] in H
+      end ;
+      MEVAL.LearnHookDefault.unfolder H ;
+      provers.ReflexivityProver.unfold_reflexivityProver H ;
+      MEVAL.Default.unfolder H ;
+      sym_evaluator s1 s2 s3 H.
+
+     Goal forall (cs : codeSpec W (settings * state)) (stn : settings) st st' SF,
+       PropX.interp cs (SepIL.SepFormula.sepFormula SF (stn, st)) -> 
+       Structured.evalCond (RvImm (natToW 0)) IL.Eq (RvImm (natToW 0)) stn st' = Some true ->
+       evalInstrs stn st (Assign Rp (RvImm (natToW 0)) :: nil) = Some st' ->
+       Regs st' Rp = natToW 0.
+     Proof.
+       intros.
+       sym_eval ltac:(isConst) empty_package simplifier.
+       intuition congruence. 
+     Abort.*)
+
+  End EmptyPackage.
+
+  Module BedrockPackage.
+    Definition bedrock_package : TypedPackage.
+    refine (
+      {| Env := {| PACK.Types := nil_Repr EmptySet_type
+        ; PACK.Funcs := bedrock_funcs_r 
+        ; PACK.Preds := fun ts => nil_Repr (SEP.Default_predicate _ _ _)
+      |}
+      ; Algos := fun ts => {| Prover := None ; Hints := None ; MemEval := None |}
+        ; Algos_correct := _
+      |}).
+    abstract (constructor; simpl; trivial).
+    Defined.
+    
+(*
+    Ltac simplifier H :=
+      match H with
+        | tt => 
+          cbv delta [
+            bedrock_package UNF.default_hintsPayload
+          ]
+        | _ => 
+          cbv delta [
+            bedrock_package UNF.default_hintsPayload
+          ] in H
+      end ;
+      MEVAL.LearnHookDefault.unfolder H ;
+      provers.ReflexivityProver.unfold_reflexivityProver H ;
+      MEVAL.Default.unfolder H ;
+      sym_evaluator H.
+*)
+  End BedrockPackage.
+
+  Module Tactics.
+
+    (** Build Packages for Provers **)
+    Ltac build_prover_pack prover ret :=
+      let res := constr:( 
+        let env :=
+          {| PACK.Types := Prover.ProverTypes prover
+           ; PACK.Funcs := fun ts => Prover.ProverFuncs prover (repr bedrock_types_r ts)
+           ; PACK.Preds := fun ts =>
+             nil_Repr (SEP.Default_predicate (repr (Prover.ProverTypes prover) (repr bedrock_types_r ts)) (tvType 0) (tvType 1))
+          |}
+        in
+        let algos ts :=
+          @Build_AllAlgos (PACK.applyTypes env ts)
+            (Some (Prover.Prover prover (PACK.applyTypes env ts)))
+            None
+            None
+        in
+        {| Env := env
+         ; Algos := algos
+         ; Algos_correct := fun ts fs ps =>
+           let types := repr bedrock_types_r ts in
+           let funcs := repr (PACK.Funcs env types) fs in
+           @Build_AllAlgos_correct types funcs ps (algos ts)
+             (@Prover.Prover_correct prover types funcs)
+             I I
+        |})
+      in
+      let res := eval simpl in res in
+      ret res.
+
+    Module ProverPackTest.
+      Require Provers.
+      (** Test **)
+      Goal TypedPackage.
+        build_prover_pack provers.TransitivityProver.TransitivityProver ltac:(fun x => refine x).
+      Defined.
+    End ProverPackTest.
+
+    Ltac build_mem_pack mem ret :=
+      match type of mem with
+        | @MEVAL.MemEvaluatorPackage ?tr ?pc ?st ?ptr ?val IL_mem_satisfies IL_ReadWord IL_WriteWord =>
+          (let res := constr:(
+             let TR := Env.repr_combine tr (MEVAL.MemEvalTypes mem) in
+             let env := 
+               {| PACK.Types := TR
+                ; PACK.Funcs := fun ts => MEVAL.MemEvalFuncs mem (Env.repr ILEnv.bedrock_types_r (Env.repr TR ts))
+                ; PACK.Preds := fun ts => MEVAL.MemEvalPreds mem (Env.repr ILEnv.bedrock_types_r (Env.repr TR ts))
+               |}
+             in
+             let algos ts :=
+               @Build_AllAlgos (PACK.applyTypes env ts) 
+                 None
+                 None 
+                 (Some (MEVAL.MemEval mem (PACK.applyTypes env ts)))
+             in
+             @Build_TypedPackage env algos 
+               (fun ts fs ps => @Build_AllAlgos_correct _ _ _ (algos ts) I I
+                 (MEVAL.MemEval_correct mem (Env.repr ILEnv.bedrock_types_r ts) _ _))) in
+           let res := eval simpl in res in
+           ret res) || fail 10000 "couldn't construct mem_package"
+        | ?T => 
+          fail 10000 "got bad type" T "expected value of type Packages.MemEvaluatorPackage"
+      end.
+
+    Definition min_types_r : Repr type :=
+      {| footprint := firstn 2 (footprint bedrock_types_r)
+       ; default := default bedrock_types_r
+      |}.
+
+    Module MemPackTest.
+
+      Goal TypedPackage.
+        pose (mem := 
+          {| MEVAL.MemEvalTypes := nil_Repr EmptySet_type
+           ; MEVAL.MemEvalFuncs := fun ts => nil_Repr (Default_signature _)
+           ; MEVAL.MemEvalPreds := fun ts => nil_Repr (SEP.Default_predicate _ _ _)
+           ; MEVAL.MemEval := fun ts => @MEVAL.Default.MemEvaluator_default _ (tvType 0) (tvType 1)
+           ; MEVAL.MemEval_correct := fun ts fs ps =>
+             @MEVAL.Default.MemEvaluator_default_correct _ _ _ _ _ _ _ _ _ _ _
+          |} : @MEVAL.MemEvaluatorPackage min_types_r (tvType 0) (tvType 1) (tvType 0) (tvType 0) 
+                   IL_mem_satisfies IL_ReadWord IL_WriteWord).
+        build_mem_pack mem ltac:(fun x => refine x).
+      Defined.
+    End MemPackTest.
+
+    (** builds a [TypedPackage] from the arguments
+     ** - [hints] is a list of separation logic hints
+     **)
+    Ltac build_hints_pack hints ret :=
+      let res := constr:(
+        let env :=
+          {| PACK.Types := PACKAGED.Types hints
+           ; PACK.Funcs := fun ts => PACKAGED.Functions hints (repr bedrock_types_r ts)
+           ; PACK.Preds := fun ts => PACKAGED.Predicates hints (repr bedrock_types_r ts) |}
+        in
+        let algos ts := 
+          @Build_AllAlgos (PACK.applyTypes env ts)
+            None 
+            (Some (PACKAGED.Hints hints ts))
+            None
+        in
+        @Build_TypedPackage env algos 
+          (fun ts fs ps => 
+            let types := repr bedrock_types_r (repr (PACKAGED.Types hints) ts) in
+            @Build_AllAlgos_correct _ _ _ (algos ts) I (PACKAGED.HintsOk hints ts fs ps) I))
+      in
+      let res := eval simpl in res in
+      ret res.
+
+    Definition bedrock_env : PACK.TypeEnv :=
+      {| PACK.Types := nil_Repr EmptySet_type
+       ; PACK.Funcs := fun ts => nil_Repr (Default_signature _)
+       ; PACK.Preds := fun ts => nil_Repr (SEP.Default_predicate _ _ _)
+      |}.
+
+    Module HintsPackTest.
+      Ltac isConst _ := true.
+      
+(*
+      Goal TypedPackage.
+        PACKAGED.prepareHints ltac:(fun x => x) W (prod IL.settings IL.state) ltac:(isConst) bedrock_env tt tt ltac:(fun v => 
+          build_hints_pack v ltac:(fun x => refine x)).
+      Defined.
+*)
+    End HintsPackTest.
+
+
+    (** given to [TypedPackage]s, combines them and passes the combined [TypedPackage]
+     ** to [k].
+     ** This tactic will fail if any of the environments are not compatible.
+     **)
+Ltac glue_pack left_pack right_pack ret :=
+  let res := constr:(
+    let l := left_pack in
+    let r := right_pack in
+    let ntypesV := Env.repr_combine (PACK.Types (Env l)) (PACK.Types (Env r)) in
+    let nfuncsV ts := 
+      Env.repr_combine (PACK.Funcs (Env l) (Env.repr ntypesV ts)) 
+                       (PACK.Funcs (Env r) (Env.repr ntypesV ts))
+    in
+    let npredsV ts :=
+      Env.repr_combine (PACK.Preds (Env l) (Env.repr ntypesV ts))
+                       (PACK.Preds (Env r) (Env.repr ntypesV ts))
+    in
+    let env :=
+      {| PACK.Types := ntypesV
+       ; PACK.Funcs := nfuncsV
+       ; PACK.Preds := npredsV
+       |}
+    in
+    let algos ts := 
+      @AllAlgos_composite (Env.repr ntypesV ts)
+                          (Algos l (Env.repr ntypesV ts))
+                          (Algos r (Env.repr ntypesV ts))
+    in
+    {| Env   := env 
+     ; Algos := algos 
+     ; Algos_correct := fun ts fs ps =>
+       AllAlgos_correct_composite (@Algos_correct l (Env.repr ntypesV ts)
+                                                    (Env.repr (nfuncsV ts) fs)
+                                                    (Env.repr (npredsV ts) ps))
+                                  (@Algos_correct r (Env.repr ntypesV ts)
+                                                    (Env.repr (nfuncsV ts) fs)
+                                                    (Env.repr (npredsV ts) ps))
+    |})
+  in ret res.
+
+(** given a tuple or list of [TypedPackage]s, this tactic combines them all and calls [k] with 
+ ** the result.
+ **)
+Ltac glue_packs packs k :=
+  match type of packs with
+    | TypedPackage => k packs
+    | _ =>
+      match packs with
+        | tt => k BedrockPackage.bedrock_package
+        | nil => k BedrockPackage.bedrock_package
+        | ?L :: ?R =>
+          glue_packs R ltac:(fun R => glue_pack L)
+        | (?L, ?R) =>
+          glue_packs L ltac:(fun L => 
+          glue_packs R ltac:(fun R => 
+            glue_pack L R k))
+      end
+  end.
+
+(** TODO: is there a way to make this more efficient? **)
+Ltac opaque_pack pack :=
+  let pack := eval hnf in pack in
+  let pack := eval simpl in pack in
+  match pack with
+    | @Build_TypedPackage ?env ?algos ?pf =>
+      refine (@Build_TypedPackage env algos _); abstract (exact pf)
+  end.
+
+Goal TypedPackage.
+  build_prover_pack provers.TransitivityProver.TransitivityProver ltac:(fun x => 
+    build_mem_pack (MEVAL.Default.package bedrock_types_r (tvType 0) (tvType 1) (tvType 0) (tvType 0) IL_mem_satisfies IL_ReadWord IL_WriteWord) ltac:(fun y =>   
+    glue_pack x y ltac:(opaque_pack))).
+Qed.
+
+(*
+Goal TypedPackage bedrock_types_r (tvType 0) (tvType 1) IL_mem_satisfies IL_ReadWord IL_WriteWord.
+  build_prover_pack Provers.TransitivityProver ltac:(fun x => 
+    build_mem_pack (MEVAL.Default.package bedrock_types_r (tvType 0) (tvType 1) (tvType 0) (tvType 0) IL_mem_satisfies IL_ReadWord IL_WriteWord) ltac:(fun y =>   
+      idtac "1" ;
+    glue_packs (x, y, y) ltac:(fun v => exact v))).
+Qed.
+*)
+  End Tactics.
+
+  Definition AlgoImpl := AllAlgos.
+  Definition AlgoProof := AllAlgos_correct.
+End ILAlgoTypes.
+
